PhysLean/StringTheory/FTheory/SU5/Quanta/IsViable.lean
@@ -36,205 +36,63 @@ open PotentialTerm ChargeSpectrum
 
 /-- For a given `I : CodimensionOneConfig` the condition on a `Quanta` for it to be
   phenomenologically viable. -/
-def IsViable (I : CodimensionOneConfig) (x : Quanta) : Prop :=
+def IsViable (x : Quanta) : Prop :=
+  /- 1. Conditions just on the charges. -/
   x.toCharges.IsComplete ∧
   ¬ x.toCharges.IsPhenoConstrained ∧
   ¬ x.toCharges.YukawaGeneratesDangerousAtLevel 1 ∧
-  AllowsTerm x.toCharges topYukawa ∧
-  x.F.toFluxesFive.NoExotics ∧
-  x.F.toFluxesFive.HasNoZero ∧
-  x.T.toFluxesTen.NoExotics ∧
-  x.T.toFluxesTen.HasNoZero ∧
-  AnomalyCancellation x.qHd x.qHu x.F x.T ∧
-  x.toCharges ∈ ofFinset I.allowedBarFiveCharges I.allowedTenCharges ∧
+  (∃ I : CodimensionOneConfig, x.toCharges ∈ ofFinset I.allowedBarFiveCharges I.allowedTenCharges) ∧
   x.F.toCharges.Nodup ∧
-  x.T.toCharges.Nodup
-
-lemma isViable_iff_expand_ofFinset (I : CodimensionOneConfig) (x : Quanta) :
-    IsViable I x ↔
-      x.toCharges.IsComplete ∧
-  ¬ x.toCharges.IsPhenoConstrained ∧
-  ¬ x.toCharges.YukawaGeneratesDangerousAtLevel 1 ∧
+  x.T.toCharges.Nodup ∧
   AllowsTerm x.toCharges topYukawa ∧
+  /- 2. Conditions just on the fluxes. -/
   x.F.toFluxesFive.NoExotics ∧
   x.F.toFluxesFive.HasNoZero ∧
   x.T.toFluxesTen.NoExotics ∧
   x.T.toFluxesTen.HasNoZero ∧
-  AnomalyCancellation x.qHd x.qHu x.F x.T ∧
-  (x.qHd.toFinset ⊆ I.allowedBarFiveCharges ∧ x.qHu.toFinset ⊆ I.allowedBarFiveCharges ∧
-      x.toCharges.Q5 ⊆ I.allowedBarFiveCharges ∧ x.toCharges.Q10 ⊆ I.allowedTenCharges)
-      ∧
-    x.F.toCharges.Nodup ∧
-    x.T.toCharges.Nodup := by
-  rw [IsViable, mem_ofFinset_iff]
-  simp [toCharges]
+  /- 3. Conditions on the combination of the charges on the flux. -/
+  AnomalyCancellation x.qHd x.qHu x.F x.T
 
-instance (I : CodimensionOneConfig) (x : Quanta) : Decidable (IsViable I x) :=
-  decidable_of_iff _ (isViable_iff_expand_ofFinset I x).symm
 
-/-!
 
-## Basic properties of charges satisfying `IsViable`
 
--/
+lemma isViable_iff_charges_mem_viableCharges (x : Quanta) :
+    IsViable x ↔
+        /- 1. Conditions just on the charges. -/
+        (∃ I, x.toCharges ∈ viableCharges I) ∧
+        x.F.toCharges.Nodup ∧
+        x.T.toCharges.Nodup ∧
+        /- 2. Conditions just on the fluxes -/
+        x.F.toFluxesFive.NoExotics ∧
+        x.F.toFluxesFive.HasNoZero ∧
+        x.T.toFluxesTen.NoExotics ∧
+        x.T.toFluxesTen.HasNoZero ∧
+        /- 3. Conditions on the fluxes and the charges. -/
+        AnomalyCancellation x.qHd x.qHu x.F x.T := by
+  rw [IsViable]
+  conv_rhs =>
+    enter [1, 1, I]
+    rw [mem_viableCharges_iff']
+  aesop
 
-lemma toCharges_five_nodup_of_isViable
-    (I : CodimensionOneConfig) (x : Quanta) (h : IsViable I x) :
-    x.F.toCharges.Nodup := h.2.2.2.2.2.2.2.2.2.2.1
+lemma isViable_iff_charges_mem_viableCharges_mem_liftCharges (x : Quanta) :
+    IsViable x ↔ (∃ I, x.toCharges ∈ viableCharges I) ∧
+      x ∈ Quanta.liftCharge x.toCharges ∧
+      AnomalyCancellation x.qHd x.qHu x.F x.T := by
+  rw [Quanta.mem_liftCharge_iff]
+  simp [toCharges_qHd, toCharges_qHu]
+  rw [FiveQuanta.mem_liftCharge_iff, TenQuanta.mem_liftCharge_iff]
+  rw [isViable_iff_charges_mem_viableCharges, ← FluxesFive.noExotics_iff_mem_elemsNoExotics,
+    ← FluxesTen.noExotics_iff_mem_elemsNoExotics]
+  aesop
 
-lemma toCharges_ten_nodup_of_isViable
-    (I : CodimensionOneConfig) (x : Quanta) (h : IsViable I x) :
-    x.T.toCharges.Nodup := h.2.2.2.2.2.2.2.2.2.2.2
-
-lemma toCharges_mem_ofFinset_of_isViable
-    (I : CodimensionOneConfig) (x : Quanta) (h : IsViable I x) :
-    x.toCharges ∈ ofFinset I.allowedBarFiveCharges I.allowedTenCharges :=
-  h.2.2.2.2.2.2.2.2.2.1
-
-lemma toFluxesFive_noExotics_of_isViable
-    (I : CodimensionOneConfig) (x : Quanta) (h : IsViable I x) :
-    x.F.toFluxesFive.NoExotics := h.2.2.2.2.1
-
-lemma toFluxesTen_noExotics_of_isViable
-    (I : CodimensionOneConfig) (x : Quanta) (h : IsViable I x) :
-    x.T.toFluxesTen.NoExotics := h.2.2.2.2.2.2.1
-
-lemma toFluxesFive_hasNoZero_of_isViable
-    (I : CodimensionOneConfig) (x : Quanta) (h : IsViable I x) :
-    x.F.toFluxesFive.HasNoZero := h.2.2.2.2.2.1
-
-lemma toFluxesTen_hasNoZero_of_isViable
-    (I : CodimensionOneConfig) (x : Quanta) (h : IsViable I x) :
-    x.T.toFluxesTen.HasNoZero := h.2.2.2.2.2.2.2.1
-
-lemma Q10_charges_mem_allowedBarTenCharges_of_isViable
-    (I : CodimensionOneConfig) (x : Quanta) (h : IsViable I x) :
-    ∀ s ∈ x.T.toCharges, s ∈ I.allowedTenCharges := by
-  have h1 := toCharges_mem_ofFinset_of_isViable I x h
-  rw [mem_ofFinset_iff] at h1
-  have h2 := h1.2.2.2
-  intro y hy
-  apply h2
-  simp [toCharges]
-  exact hy
-
-lemma Q5_charges_mem_allowedBarFiveCharges_of_isViable
-    (I : CodimensionOneConfig) (x : Quanta) (h : IsViable I x) :
-    ∀ s ∈ x.F.toCharges, s ∈ I.allowedBarFiveCharges := by
-  have h1 := toCharges_mem_ofFinset_of_isViable I x h
-  rw [mem_ofFinset_iff] at h1
-  have h2 := h1.2.2.1
-  intro y hy
-  apply h2
-  simp [toCharges]
-  exact hy
-
-lemma topYukawa_allowsTerm_of_isViable
-    (I : CodimensionOneConfig) (x : Quanta) (h : IsViable I x) :
-    AllowsTerm x.toCharges topYukawa := by
-  exact h.2.2.2.1
-
-lemma not_isPhenoConstrained_of_isViable
-    (I : CodimensionOneConfig) (x : Quanta) (h : IsViable I x) :
-    ¬ x.toCharges.IsPhenoConstrained := by
-  exact h.2.1
-
-lemma toCharges_isComplete_of_isViable
-    (I : CodimensionOneConfig) (x : Quanta) (h : IsViable I x) :
-    x.toCharges.IsComplete := by
-  exact h.1
-
-lemma anomalyCancellation_of_isViable
-    (I : CodimensionOneConfig) (x : Quanta) (h : IsViable I x) :
-    AnomalyCancellation x.qHd x.qHu x.F x.T := by
-  exact h.2.2.2.2.2.2.2.2.1
-
-lemma reduce_five_eq_self_of_isViable
-    (I : CodimensionOneConfig) (x : Quanta) (h : IsViable I x) :
-    x.F.reduce = x.F := by
-  match x with
-  | ⟨qHd, qHu, F, T⟩ =>
-    simp only
-    refine FiveQuanta.reduce_eq_self_of_ofCharges_nodup F ?_
-    simp [IsViable] at h
-    simp_all
-
-lemma reduce_ten_eq_self_of_isViable
-    (I : CodimensionOneConfig) (x : Quanta) (h : IsViable I x) :
-    x.T.reduce = x.T := by
-  match x with
-  | ⟨qHd, qHu, F, T⟩ =>
-    simp only
-    refine TenQuanta.reduce_eq_self_of_ofCharges_nodup T ?_
-    simp [IsViable] at h
-    simp_all
-
-lemma reduce_eq_self_of_isViable
-    (I : CodimensionOneConfig) (x : Quanta) (h : IsViable I x) :
-    x.reduce = x := by
-  match x with
-  | ⟨qHd, qHu, F, T⟩ =>
-    simp [reduce]
-    constructor
-    · exact reduce_five_eq_self_of_isViable I _ h
-    · exact reduce_ten_eq_self_of_isViable I _ h
-
-lemma mem_ofChargesExpand_of_isViable
-    (I : CodimensionOneConfig) (x : Quanta) (h : IsViable I x) :
-    x ∈ (ofChargesExpand x.toCharges).map reduce := by
-  simp [ofChargesExpand]
-  have h_five : x.F ∈ (FiveQuanta.ofChargesExpand x.F.toCharges.toFinset).map
-      FiveQuanta.reduce := by
-    refine (FiveQuanta.mem_ofChargesExpand_map_reduce_iff x.F.toCharges.toFinset x.F).mpr ?_
-    · refine ⟨?_, rfl, ?_⟩
-      · rw [← SU5.FluxesFive.noExotics_iff_mem_elemsNoExotics]
-        refine ⟨?_, ?_⟩
-        · exact toFluxesFive_noExotics_of_isViable I x h
-        · exact toFluxesFive_hasNoZero_of_isViable I x h
-      · exact reduce_five_eq_self_of_isViable I x h
-  have h_ten : x.T ∈ (TenQuanta.ofChargesExpand x.T.toCharges.toFinset).map
-      TenQuanta.reduce := by
-    refine (TenQuanta.mem_ofChargesExpand_map_reduce_iff x.T.toCharges.toFinset x.T).mpr ?_
-    · refine ⟨?_, rfl, ?_⟩
-      · rw [← SU5.FluxesTen.noExotics_iff_mem_elemsNoExotics]
-        refine ⟨?_, ?_⟩
-        · exact toFluxesTen_noExotics_of_isViable I x h
-        · exact toFluxesTen_hasNoZero_of_isViable I x h
-      · exact reduce_ten_eq_self_of_isViable I x h
-  rw [Multiset.mem_map] at h_five h_ten
-  obtain ⟨F, F_mem, hF⟩ := h_five
-  obtain ⟨T, T_mem, hT⟩ := h_ten
-  refine ⟨F, ⟨F_mem, ⟨T, ⟨T_mem, ?_⟩⟩⟩⟩
-  simp_all [reduce, toCharges]
-
-lemma toCharges_isAnomalyFree_of_isViable
-    (I : CodimensionOneConfig) (x : Quanta) (h : IsViable I x) :
-    IsAnomalyFree x.toCharges := by
-  simp only [IsAnomalyFree]
-  have h1 := mem_ofChargesExpand_of_isViable I x h
-  rw [Multiset.mem_map] at h1
-  obtain ⟨y, y_mem, rfl⟩ := h1
-  use y
-  refine ⟨?_, ?_⟩
-  · exact y_mem
-  · have acc := anomalyCancellation_of_isViable I _ h
-    simp only [AnomalyCancellation, reduce] at acc
-    rw [FiveQuanta.anomalyCoefficent_of_reduce, TenQuanta.anomalyCoefficent_of_reduce] at acc
-    simp [AnomalyCancellation]
-    rw [← acc]
-
-lemma toCharges_mem_viableCharges_filter_isAnomalyFree_of_isViable
-    (I : CodimensionOneConfig) (x : Quanta) (h : IsViable I x) :
-    x.toCharges ∈ (viableCharges I).filter IsAnomalyFree := by
-  simp only [Multiset.mem_filter]
-  apply And.intro
-  · refine (mem_viableCharges_iff ?_).mpr ⟨?_, ?_, ?_, ?_⟩
-    · exact toCharges_mem_ofFinset_of_isViable I x h
-    · exact topYukawa_allowsTerm_of_isViable I x h
-    · exact not_isPhenoConstrained_of_isViable I x h
-    · exact h.2.2.1
-    · exact toCharges_isComplete_of_isViable I x h
-  · exact toCharges_isAnomalyFree_of_isViable I x h
+lemma isViable_iff_filter (x : Quanta) :
+    IsViable x ↔ (∃ I, x.toCharges ∈ (viableCharges I).filter IsAnomalyFree) ∧
+      x ∈ Quanta.liftCharge x.toCharges
+      ∧ AnomalyCancellation x.qHd x.qHu x.F x.T := by
+  rw [isViable_iff_charges_mem_viableCharges_mem_liftCharges]
+  simp [IsAnomalyFree]
+  aesop
 
 /-!
 
@@ -242,58 +100,43 @@ lemma toCharges_mem_viableCharges_filter_isAnomalyFree_of_isViable
 -/
 
 /-- Given a `CodimensionOneConfig` the `Quanta` which statisfy the condition `IsViable`. -/
-def viableElems : CodimensionOneConfig → Multiset Quanta
-  | .same => {⟨some 2, some (-2), {(-1, ⟨1, 2⟩), (1, ⟨2, -2⟩)}, {(-1, ⟨3, 0⟩)}⟩,
-      ⟨some 2, some (-2), {(-1, ⟨0, 2⟩), (1, ⟨3, -2⟩)}, {(-1, ⟨3, 0⟩)}⟩,
-      ⟨some (-2), some 2, {(-1, ⟨2, -2⟩), (1, ⟨1, 2⟩)}, {(1, ⟨3, 0⟩)}⟩,
-      ⟨some (-2), some 2, {(-1, ⟨3, -2⟩), (1, ⟨0, 2⟩)}, {(1, ⟨3, 0⟩)}⟩}
-  | .nearestNeighbor => {⟨some 6, some (-14), {(-9, ⟨1, 2⟩), (1, ⟨2, -2⟩)}, {(-7, ⟨3, 0⟩)}⟩,
+def viableElems :  Multiset Quanta :=
+  {⟨some 2, some (-2), {(-1, ⟨1, 2⟩), (1, ⟨2, -2⟩)}, {(-1, ⟨3, 0⟩)}⟩,
+    ⟨some 2, some (-2), {(-1, ⟨0, 2⟩), (1, ⟨3, -2⟩)}, {(-1, ⟨3, 0⟩)}⟩,
+    ⟨some (-2), some 2, {(-1, ⟨2, -2⟩), (1, ⟨1, 2⟩)}, {(1, ⟨3, 0⟩)}⟩,
+    ⟨some (-2), some 2, {(-1, ⟨3, -2⟩), (1, ⟨0, 2⟩)}, {(1, ⟨3, 0⟩)}⟩,
+    ⟨some 6, some (-14), {(-9, ⟨1, 2⟩), (1, ⟨2, -2⟩)}, {(-7, ⟨3, 0⟩)}⟩,
     ⟨some 6, some (-14), {(-9, ⟨0, 2⟩), (1, ⟨3, -2⟩)}, {(-7, ⟨3, 0⟩)}⟩}
-  | .nextToNearestNeighbor => {}
 
-lemma isViable_of_mem_viableElems
-    (I : CodimensionOneConfig) (x : Quanta) (h : x ∈ viableElems I) :
-    IsViable I x := by
-  revert x I
+
+lemma isViable_of_mem_viableElems (x : Quanta) (h : x ∈ viableElems) :
+    IsViable x := by
+  rw [isViable_iff_charges_mem_viableCharges_mem_liftCharges]
+  revert x
   decide
 
-lemma viableElems_card_eq (I : CodimensionOneConfig) :
-    (viableElems I).card = match I with
-    | .same => 4
-    | .nearestNeighbor => 2
-    | .nextToNearestNeighbor => 0 := by
-  cases I <;> rfl
-
-lemma mem_viableElems_of_isViable
-    (I : CodimensionOneConfig) (x : Quanta) (h : IsViable I x) :
-    x ∈ viableElems I := by
-  have hx := mem_ofChargesExpand_of_isViable I x h
-  have hc := toCharges_mem_viableCharges_filter_isAnomalyFree_of_isViable I x h
-  rw [viable_anomalyFree] at hc
-  generalize x.toCharges = c at hc hx
-  fin_cases I
-  all_goals
-  · dsimp at hc
-    fin_cases hc
-    all_goals
-    · revert h
-      revert x
-      decide
-
-lemma isViable_iff_mem_viableElems
-    (I : CodimensionOneConfig) (x : Quanta) :
-    IsViable I x ↔ x ∈ viableElems I := by
+lemma isViable_iff_mem_viableElems (x : Quanta) :
+    x.IsViable ↔ x ∈ viableElems := by
   constructor
-  · exact mem_viableElems_of_isViable I x
-  · exact isViable_of_mem_viableElems I x
+  · intro h
+    rw [isViable_iff_filter] at h
+    obtain ⟨⟨I, hc⟩, hl, ha⟩ := h
+    generalize x.toCharges = c at *
+    revert ha
+    revert x
+    rw [viable_anomalyFree] at hc
+    revert c
+    revert I
+    decide
+  · exact isViable_of_mem_viableElems x
 
 /-- Every viable Quanta regenerates a dangerous coupling at two insertions of the Yukawa
   singlets. -/
 lemma yukawaSingletsRegenerateDangerousInsertion_two_of_isViable
-    (I : CodimensionOneConfig) (x : Quanta) (h : IsViable I x) :
+    (x : Quanta) (h : IsViable x) :
     (toCharges x).YukawaGeneratesDangerousAtLevel 2 := by
   rw [isViable_iff_mem_viableElems] at h
-  revert I x
+  revert x
   decide
 
 end Quanta
